updating

coq/Test_5.v
@@ -280,4 +280,442 @@ Definition mdl : llvm_module :=
     ]
   ).
 
+Definition gs := empty_smt_store.
 
+Definition s_ls_0 := empty_smt_store.
+Definition s_stk_0 : list sym_frame := [].
+Definition s_symbolics_0 : list string := [].
+Definition s_pc_0 := SMT_True.
+Definition s_0 := mk_sym_state
+  (mk_inst_counter (Name "main") (Name "entry") 0)
+  inst_0
+  [inst_1; inst_2; inst_3; inst_4]
+  None
+  s_ls_0
+  s_stk_0
+  gs
+  s_symbolics_0
+  s_pc_0
+  mdl
+.
+
+Definition s_ls_1 := ((Name "call") !-> Some (SMT_Var_I32 (fresh_name s_symbolics_0)); s_ls_0).
+Definition s_stk_1 := s_stk_0.
+Definition s_symbolics_1 := extend_names s_symbolics_0.
+Definition s_pc_1 := s_pc_0.
+Definition s_1 := mk_sym_state
+  (mk_inst_counter (Name "main") (Name "entry") 1)
+  inst_1
+  [inst_2; inst_3; inst_4]
+  None
+  s_ls_1
+  s_stk_1
+  gs
+  s_symbolics_1
+  s_pc_1
+  mdl
+.
+
+Definition s_ls_2 := ((Name "cmp") !-> Some (SMT_CmpOp SMT_Sgt (SMT_Var_I32 (fresh_name s_symbolics_0)) (SMT_Const_I32 (Int32.repr 7))); s_ls_1).
+Definition s_stk_2 := s_stk_1.
+Definition s_symbolics_2 := s_symbolics_1.
+Definition s_pc_2 := s_pc_1.
+Definition s_2 := mk_sym_state
+  (mk_inst_counter (Name "main") (Name "entry") 2)
+  inst_2
+  [inst_3; inst_4]
+  None
+  s_ls_2
+  s_stk_2
+  gs
+  s_symbolics_2
+  s_pc_2
+  mdl
+.
+
+Definition s_ls_3 := s_ls_2.
+Definition s_stk_3 := s_stk_2.
+Definition s_symbolics_3 := s_symbolics_2.
+Definition s_pc_3 := (SMT_BinOp SMT_And s_pc_2 (SMT_CmpOp SMT_Sgt (SMT_Var_I32 (fresh_name s_symbolics_0)) (SMT_Const_I32 (Int32.repr 7)))).
+Definition s_3 := mk_sym_state
+  (mk_inst_counter (Name "main") (Name "entry") 3)
+  inst_3
+  [inst_4]
+  None
+  s_ls_3
+  s_stk_3
+  gs
+  s_symbolics_3
+  s_pc_3
+  mdl
+.
+
+Definition s_ls_4 := ((Name "cmp1") !-> Some (SMT_CmpOp SMT_Sgt (SMT_Var_I32 (fresh_name s_symbolics_0)) (SMT_Const_I32 (Int32.repr 3))); s_ls_3).
+Definition s_stk_4 := s_stk_3.
+Definition s_symbolics_4 := s_symbolics_3.
+Definition s_pc_4 := s_pc_3.
+Definition s_4 := mk_sym_state
+  (mk_inst_counter (Name "main") (Name "entry") 4)
+  inst_4
+  []
+  None
+  s_ls_4
+  s_stk_4
+  gs
+  s_symbolics_4
+  s_pc_4
+  mdl
+.
+
+Definition s_ls_5 := s_ls_4.
+Definition s_stk_5 := s_stk_4.
+Definition s_symbolics_5 := s_symbolics_4.
+Definition s_pc_5 := s_pc_4.
+Definition s_5 := mk_sym_state
+  (mk_inst_counter (Name "main") (Name "if.then") 5)
+  inst_5
+  []
+  (Some (Name "entry"))
+  s_ls_5
+  s_stk_5
+  gs
+  s_symbolics_5
+  s_pc_5
+  mdl
+.
+
+Definition s_ls_6 := s_ls_5.
+Definition s_stk_6 := s_stk_5.
+Definition s_symbolics_6 := s_symbolics_5.
+Definition s_pc_6 := s_pc_5.
+Definition s_6 := mk_sym_state
+  (mk_inst_counter (Name "main") (Name "if.end") 7)
+  inst_7
+  []
+  (Some (Name "if.then"))
+  s_ls_6
+  s_stk_6
+  gs
+  s_symbolics_6
+  s_pc_6
+  mdl
+.
+
+Definition s_ls_7 := s_ls_6.
+Definition s_stk_7 := s_stk_6.
+Definition s_symbolics_7 := s_symbolics_6.
+Definition s_pc_7 := (SMT_BinOp SMT_And s_pc_2 (SMT_Not (SMT_CmpOp SMT_Sgt (SMT_Var_I32 (fresh_name s_symbolics_0)) (SMT_Const_I32 (Int32.repr 7))))).
+Definition s_7 := mk_sym_state
+  (mk_inst_counter (Name "main") (Name "if.then") 6)
+  inst_6
+  []
+  (Some (Name "entry"))
+  s_ls_7
+  s_stk_7
+  gs
+  s_symbolics_7
+  s_pc_7
+  mdl
+.
+
+Definition t_7 := t_leaf s_7.
+Definition t_6 := t_leaf s_6.
+Definition t_5 := t_subtree s_5 [t_6].
+Definition t_4 := t_subtree s_4 [t_5; t_7].
+Definition t_3 := t_subtree s_3 [t_4].
+Definition t_2 := t_subtree s_2 [t_3].
+Definition t_1 := t_subtree s_1 [t_2].
+Definition t_0 := t_subtree s_0 [t_1].
+
+Lemma L_6 : safe_et_opt t_6.
+Proof.
+apply Safe_Leaf_Ret.
+Qed.
+
+Lemma L_5 : safe_et_opt t_5.
+Proof.
+{
+  apply Safe_Subtree.
+  {
+    apply LAUX_not_error_unconditional_br.
+  }
+  {
+    intros s Hse.
+    {
+      left.
+      exists (t_6).
+      split.
+      {
+        simpl.
+        left.
+        reflexivity.
+      }
+      {
+        split.
+        {
+          apply L_6.
+        }
+        {
+          simpl.
+          inversion Hse; subst.
+          (* TODO use a specific lemma *)
+          inversion H10; subst.
+          inversion H11; subst.
+          inversion H12; subst.
+          apply EquivSymState.
+          { apply equiv_smt_store_refl. }
+          { apply equiv_sym_stack_refl. }
+          { apply equiv_smt_store_refl. }
+          { apply equiv_smt_expr_refl. }
+        }
+      }
+    }
+  }
+}
+Qed.
+
+
+Lemma L_4 : safe_et_opt t_4.
+Proof.
+{
+  apply Safe_Subtree.
+  {
+    apply LAUX_not_error_br.
+  }
+  {
+    intros s Hse.
+    inversion Hse; subst.
+    {
+      left.
+      exists (t_5).
+      split.
+      {
+        simpl.
+        left.
+        reflexivity.
+      }
+      {
+        split.
+        {
+          apply L_5.
+        }
+        {
+          simpl.
+          inversion H13; subst.
+          inversion H14; subst.
+          inversion H15; subst.
+          apply EquivSymState.
+          { apply equiv_smt_store_refl. }
+          { apply equiv_sym_stack_refl. }
+          { apply equiv_smt_store_refl. }
+          {
+            inversion H12; subst.
+            (* TODO: simplify lemma *)
+            admit.
+          }
+        }
+      }
+    }
+    {
+      right.
+      apply Unsat_State.
+      inversion H12; subst.
+      (* TODO: add axiom *)
+      admit.
+    }
+  }
+}
+Admitted.
+
+Lemma L_3 : safe_et_opt t_3.
+Proof.
+{
+  apply Safe_Subtree.
+  {
+    apply LAUX_not_error_instr_op.
+  }
+  {
+    intros s Hse.
+    {
+      left.
+      exists (t_4).
+      split.
+      {
+        simpl.
+        left.
+        reflexivity.
+      }
+      {
+        split.
+        {
+          apply L_4.
+        }
+        {
+          simpl.
+          inversion Hse; subst.
+          apply EquivSymState.
+          {
+            simpl in H13.
+            apply LAUX_1 with
+              (se1 := (sym_eval_icmp Sgt (SMT_Var_I32 (fresh_name s_symbolics_0))
+           (SMT_Const_I32 (Int32.repr 3))))
+              (se2 := se).
+            { assumption. }
+            { admit. } (* simplify lemma *)
+          }
+          { apply equiv_sym_stack_refl. }
+          { apply equiv_smt_store_refl. }
+          { apply equiv_smt_expr_refl. }
+        }
+      }
+    }
+  }
+}
+Admitted.
+
+Lemma L_2 : safe_et_opt t_2.
+Proof.
+{
+  apply Safe_Subtree.
+  {
+    apply LAUX_not_error_void_call.
+    intros H.
+    discriminate H.
+  }
+  {
+    intros s Hse.
+    {
+      left.
+      exists (t_3).
+      split.
+      {
+        simpl.
+        left.
+        reflexivity.
+      }
+      {
+        split.
+        {
+          apply L_3.
+        }
+        {
+          simpl.
+          inversion Hse; subst.
+          (* TODO: add missing declarations *)
+          inversion H14.
+        }
+      }
+    }
+  }
+}
+Admitted.
+
+Lemma L_1 : safe_et_opt t_1.
+Proof.
+{
+  apply Safe_Subtree.
+  {
+    apply LAUX_not_error_instr_op.
+  }
+  {
+    intros s Hse.
+    {
+      left.
+      exists (t_2).
+      split.
+      {
+        simpl.
+        left.
+        reflexivity.
+      }
+      {
+        split.
+        {
+          apply L_2.
+        }
+        {
+          simpl.
+          inversion Hse; subst.
+          apply EquivSymState.
+          {
+            simpl in H13.
+            apply LAUX_1 with
+              (se1 := (sym_eval_icmp Sgt (SMT_Var_I32 (fresh_name s_symbolics_0))
+           (SMT_Const_I32 (Int32.repr 7))))
+              (se2 := se).
+            { assumption. }
+            { admit. } (* simplify lemma *)
+          }
+          { apply equiv_sym_stack_refl. }
+          { apply equiv_smt_store_refl. }
+          { apply equiv_smt_expr_refl. }
+        }
+      }
+    }
+  }
+}
+Admitted.
+
+Lemma L_0 : safe_et_opt t_0.
+Proof.
+{
+  apply Safe_Subtree.
+  {
+    apply LAUX_not_error_call.
+  }
+  {
+    intros s Hse.
+    {
+      left.
+      exists (t_1).
+      split.
+      {
+        simpl.
+        left.
+        reflexivity.
+      }
+      {
+        split.
+        {
+          apply L_1.
+        }
+        {
+          simpl.
+          inversion Hse; subst.
+          (* find_function_by_exp does not return None *)
+          (* TODO: avoid *)
+          { inversion H16. }
+          (* find_function_by_exp returns None *)
+          {
+            apply EquivSymState.
+            { apply equiv_smt_store_refl. }
+            { apply equiv_sym_stack_refl. }
+            { apply equiv_smt_store_refl. }
+            { apply equiv_smt_expr_refl. }
+          }
+        }
+      }
+    }
+  }
+}
+Admitted.
+
+Theorem program_safe : is_safe_program mdl (Name "main").
+Proof.
+{
+  destruct t_0 as [r | r l] eqn:E.
+  {
+    discriminate E.
+  }
+  {
+    apply completeness_via_et with (init_s := s_0) (l := l).
+    { admit. }
+    { reflexivity. }
+    {
+      inversion E; subst.
+      rewrite <- E.
+      apply L_0.
+    }
+  }
+}
+Admitted.
